
% EBVC
\begin{aligned}
    r_b^i(X_v) &= A \sum_{x \in X_v} f\left(\theta_x - \theta_h \mid \hat \theta_i, \sigma_\theta (\hat d_i)\right) \times f\left(d_x\mid \hat d_i, \sigma_d\right)
    \\
    \sigma_\theta (\hat d_i) &= \sigma_0 + c \hat d_i
\end{aligned}

% ABVC
\begin{aligned}
    r_b^i(X) &= A \sum_{x \in X} f\left(\theta_x\mid \hat \theta_i, \sigma_\theta (\hat d_i)\right) \times f\left(d_x\mid \hat d_i, \sigma_d\right)
    \\
    \sigma_\theta (\hat d_i) &= \sigma_0 + c \hat d_i
\end{aligned}

% Place Cells
\begin{aligned}
    \tau_p \frac{\partial }{\partial t} r_p^{i} &= -r_p^{i} + \frac{\left[I - \delta \right ]_+}{\gamma \sum_i r_p^{i}}
    \\
    I &= W_g r_g + W_b r_b
    \\
    \tau_\delta \frac{\mathrm{d} }{\mathrm{d} t}\delta &= -\delta + \left \langle I \right \rangle + c Std(I)
    \\
    W_k^{ij} &= \left[W_k^{ij} + \eta_k r_p^{i} \left(r_k^{j} - \left \langle r_k \right \rangle\right)\right]_+, \hspace{5mm} k \in \{g, b\}
\end{aligned}
